theorems/experiments/ir/Basic.lean
@@ -1,0 +1,68 @@
+import theorems.iN
+
+inductive IR : Nat → Type where
+  | var (id : Nat) : IR idx
+  | const (val : Nat) : IR idx
+  | const_poison : IR idx
+
+  | add (lhs rhs : IR idx) : IR idx
+  | addNsw (lhs rhs : IR idx) : IR idx
+deriving BEq, Repr, Lean.ToExpr
+
+deriving instance BEq for iN
+
+structure PackediN where
+  {n : Nat}
+  x : iN n
+deriving BEq
+
+structure PackedIR where
+  {idx : Nat}
+  ir : IR idx
+deriving Repr
+
+def PackediN.truncate (pack : PackediN) (n : Nat) : iN n :=
+  match pack.x with
+  | poison => poison
+  | bitvec a => a.truncate n
+
+abbrev Assignment := Lean.RArray PackediN
+abbrev WidthAssignment := Lean.RArray Nat
+
+namespace IR
+
+@[reducible]
+def eval (ξ : WidthAssignment) (σ : Assignment) : IR idx → iN (ξ.get idx)
+  | var id =>
+    let pack := σ.get id
+    /- h is always true, this if is for totality -/
+    if h : pack.n = (ξ.get idx) then
+      h ▸ pack.x
+    else
+      pack.truncate (ξ.get idx)
+
+  | const val => bitvec val
+  | const_poison => poison
+
+  | add lhs rhs => iN.add (eval ξ σ lhs) (eval ξ σ rhs)
+  | addNsw lhs rhs => iN.addNsw (eval ξ σ lhs) (eval ξ σ rhs)
+
+  /- | add lhs rhs => iN.add (eval σ lhs) (eval σ rhs)
+  | addNsw lhs rhs => iN.addNsw (eval σ lhs) (eval σ rhs)
+  | addNuw lhs rhs => iN.addNuw (eval σ lhs) (eval σ rhs)
+  | addNw lhs rhs => iN.addNw (eval σ lhs) (eval σ rhs) -/
+
+end IR
+
+
+/--
+For the implementation to optimise, it needs to know whether or not the width assignment respect the `valid` prop.
+--/
+structure Rule where
+  valid : WidthAssignment → Bool
+
+  impl : {idx : Nat} → IR idx → IR idx
+
+  wf : ∀ (ξ : WidthAssignment) (ξvalid : valid ξ) (σ : Assignment) (lhs : IR idx),
+    let rhs := impl lhs
+    (IR.eval ξ σ lhs) ~> (IR.eval ξ σ rhs)
