theorems/experiments/ir/Reify.lean
@@ -1,0 +1,214 @@
+import theorems.experiments.ir.Basic
+
+import Lean
+import Qq
+open Lean Elab Meta
+open Qq
+
+/- ir = reify expr        (IR.eval ir = expr) -/
+
+
+structure ReifyEnv where
+  /- "evals at assignments" -/
+  ξQ : Q(WidthAssignment)
+  σQ : Q(Assignment) /- varId → iN ?? -/
+
+  /- FVarId → varId -/
+  σMap : Std.HashMap FVarId Nat
+
+def ReifyEnv.of' (assignment : Array (FVarId × Nat)) (width_assignment : Array FVarId)
+  (h : 0 < assignment.size) (h' : 0 < width_assignment.size) : MetaM ReifyEnv := do
+  let assignment' : RArray (FVarId × Nat) :=
+    RArray.ofArray assignment h
+
+  let width_assignment' : RArray FVarId :=
+    RArray.ofArray width_assignment h'
+
+  have ξQ : Q(WidthAssignment) :=
+    ← width_assignment'.toExpr q(Nat) fun (fvar : FVarId) => mkFVarEx fvar
+
+  have σQ : Q(Assignment) :=
+    ← assignment'.toExpr q(PackediN) fun (⟨x, idx⟩ : FVarId × Nat) =>
+      /- we want iN (ξ.get idx) -/
+      /- ⟨ξ.get idx, x⟩ -/
+
+      have idxQ : Q(Nat) := toExpr idx
+
+      have xQ : Q(iN (($ξQ).get $idxQ)) := mkFVarEx x
+      have fid : Q(PackediN) := q(@PackediN.mk (($ξQ).get $idxQ) $xQ)
+      fid
+
+  let σMap := Std.HashMap.ofArray assignment
+  return ⟨ξQ, σQ, σMap⟩
+
+/- accepts expressions of the form
+  `fun {n} ... {m} (x : iN n) ... (z : iN m) : iN n => ...` -/
+/- entire expression is iN (ξ.get result_idx) -/
+def ReifyEnv.of (fvars : Array Expr) (body : Expr) : MetaM (Nat × ReifyEnv) := do
+  /- map each type iN n -> idx of WidthAssignment -/
+  /- these are fvars being m, n, ... -/
+  let mut width_assignment : Array FVarId := #[]
+
+  /- map each expr x -> idx of Assignment -/
+  let mut assignment : Array (FVarId × Nat) := #[]
+
+  for fvar in fvars do
+    /- https://github.com/leanprover-community/quote4/issues/36 -/
+    let fvar_type ← inferType fvar
+
+    match_expr fvar_type with
+    | Nat =>
+      width_assignment := width_assignment.push fvar.fvarId!
+    | iN nv =>
+
+      /- n should be an fvar, if we have for example (x : iN 32),
+        we should encode it as ∀n : Nat, n = 32 → ... inside valid.
+        this is unhandled for now -/
+      let some assignmentIdx := width_assignment.findIdx? (fun widthFvar => widthFvar == nv.fvarId!)
+        | throwError "reifyExpr: unbound, not previous free variable in Nat"
+
+      assignment := assignment.push (fvar.fvarId!, assignmentIdx)
+    | _ => throwError "reifyExpr: unsupported type"
+
+  if h : ¬0 < assignment.size then
+    unreachable!
+  else if h' : ¬0 < width_assignment.size then
+    unreachable!
+  else
+
+  let body_type ← inferType body
+  let resultIdx ← match_expr body_type with
+  | iN nv =>
+
+    let some assignmentIdx := width_assignment.findIdx? (fun widthFvar => widthFvar == nv.fvarId!)
+      | throwError "reifyExpr: unbound, not previous free variable in Nat"
+
+    pure assignmentIdx
+  | _ => throwError "reifyExpr: unsupported body type {body_type}"
+
+  let env ← ReifyEnv.of' assignment width_assignment
+    (by exact Decidable.of_not_not h) (by exact Decidable.of_not_not h')
+
+  return ⟨resultIdx, env⟩
+
+abbrev M := ReaderT ReifyEnv MetaM
+
+namespace M
+
+def run' (env : ReifyEnv) (m : M α) : MetaM α :=
+  m.run env
+
+end M
+
+
+structure ReifiedIR (idx : Nat) where
+  irExpr : IR idx
+  originalExpr : Expr
+
+  /- proof that IR.eval irExpr = originalExpr, or by rfl if none  -/
+  proof : M (Option Expr)
+
+namespace ReifiedIR
+
+def mkEvalIR (idx : Nat) (expr : Q(IR $idx)) : M Expr := do
+  let st ← read
+  return q(IR.eval $(st.ξQ) $(st.σQ) $expr)
+
+end ReifiedIR
+
+theorem reflect_poison_eval_poison {idx ξ σ}
+  : IR.eval ξ σ (IR.const_poison : IR idx) = (poison : iN (ξ.get idx)) := rfl
+
+/- theorem reflect_var_eval_var {idx ξ σ id}
+  : IR.eval ξ σ (IR.var id : IR idx) = (σ.get id : iN (ξ.get idx)) := rfl -/
+
+partial def reifyIRExpr (idx : Nat) (body : Expr) : M (ReifiedIR idx) := do
+  match_expr body with
+  | iN.poison _ =>
+    let ⟨ξQ, σQ, _⟩ ← read
+
+    --have irExpr : Q(IR $idx) := toExpr $ IR.const_poison
+    let proof := pure q(@reflect_poison_eval_poison $idx $ξQ $σQ)
+    return ⟨IR.const_poison, body, proof⟩
+
+  /- | iN.bitvec _ e =>
+    if let some (v, _) := (← getOfNatValue? e ``BitVec) then
+      return IR.const v
+
+    throwError "reifyIRExpr: unsupported bitvec expression {body}"
+
+  | iN.add _ lhs rhs =>
+    let lhs_ir ← reifyIRExpr idx assignment lhs
+    let rhs_ir ← reifyIRExpr idx assignment rhs
+    return IR.add lhs_ir rhs_ir
+  | iN.addNsw _ lhs rhs =>
+    let lhs_ir ← reifyIRExpr idx assignment lhs
+    let rhs_ir ← reifyIRExpr idx assignment rhs
+    return IR.addNsw lhs_ir rhs_ir -/
+  | _ =>
+    let ⟨_, _, σMap⟩ ← read
+
+    if let some fvarid := body.fvarId? then
+      let some varId := σMap.get? fvarid
+        | throwError "reifyIRExpr: unbound free variable {body}"
+
+      return ⟨IR.var varId, body, pure none⟩
+
+      --return IR.var varId
+
+    throwError "reifyIRExpr: unsupported expression {body}"
+
+elab "⟪" t:term "⟫" : term => do
+  let t ← Term.elabTerm t none
+  lambdaTelescope t fun fvars body => do
+    /- body : iN (ξ.get resultIdx) -/
+    let (resultIdx, env) := ← ReifyEnv.of fvars body; M.run' env do
+
+
+    let ir ← (reifyIRExpr resultIdx body).run env
+
+    logInfo m!"ir: {repr ir.irExpr}"
+    logInfo m!"proof: {← ir.proof}"
+
+    have irExpr : Q(IR $resultIdx) := toExpr ir.irExpr
+    let evalExpr : Expr ← ReifiedIR.mkEvalIR resultIdx irExpr
+    /- IR.eval ... =  -/
+
+    /- logInfo m!"print: {← isDefEq evalExpr}"
+ -/
+
+    if (← withTransparency (.all) <| isDefEq evalExpr body) then
+      logInfo "yes"
+
+    /- if not (← isDefEq evalExpr body) then
+      logInfo "why?" -/
+
+    let expr ← mkEq evalExpr body
+    logInfo m!"expr: {expr}"
+    check expr
+
+    return t
+
+--#eval ⟪fun {n} (x : iN n) => x +nsw x⟫
+#eval ⟪fun {n} (x : iN n) => x⟫
+
+theorem test {n} (x : iN n)
+    : IR.eval (RArray.leaf n) (RArray.leaf { n := (RArray.leaf n).get 0, x := x }) (IR.var 0 : IR 0) = x := by
+
+
+
+  rfl
+
+theorem test' {n} (x : iN n)
+    : IR.eval (RArray.leaf n) (RArray.leaf { n := (RArray.leaf n).get 0, x := x }) (IR.var 0 : IR 0) =
+
+      (let pack := (RArray.leaf { n := (RArray.leaf n).get 0, x := x } : Assignment).get 0
+      /- h is always true, this if is for totality -/
+      if h : pack.n = ((RArray.leaf n).get 0) then
+        h ▸ pack.x
+      else
+        pack.truncate ((RArray.leaf n).get 0)) := by
+
+  rfl
+
+#print test
